Did course work

Tree.v
@@ -9,9 +9,10 @@ Inductive BinaryTree (T : Type) : Type :=
     | Node : BinaryTree T -> BinaryTree T -> T -> BinaryTree T -> BinaryTree T
     .
 
-Check (Nill).
 Check (Nill nat).
 Check (Node (Nill nat) (Nill nat) 5 (Nill nat)).
+Check (Node (Nill nat) (Nill nat) 5 
+      (Node (Nill nat) (Nill nat) 7 (Nill nat))).
 
 (* ========================= *)
 (* Functions of BinaryTree T *)
@@ -28,6 +29,19 @@ Definition Rst {T} (tree : BinaryTree T) : BinaryTree T :=
   | Nill => Nill T
   | Node _ _ _ Right => Right
   end.
+
+Notation null := (Nill nat).
+Notation "l -| v |- r" := (Node (Nill nat) l v r) (at level 43, left associativity).
+Notation "@ v " := (null -| v |- null) (at level 43, left associativity).
+
+Eval compute in (Lst null).
+Eval compute in (Rst null).
+
+Eval compute in (Lst (@5)).
+Eval compute in (Rst (@5)).
+
+Eval compute in (Lst ((@3) -| 5 |- (@7))).
+Eval compute in (Rst ((@3) -| 5 |- (@7))).
 
 Fixpoint nodes {T} (tree : BinaryTree T) : seq T := 
   match tree with
@@ -53,15 +67,13 @@ Qed.
 Lemma height_empty_tree : forall {T} (tree : BinaryTree T),
   height tree = 0 <-> tree = Nill T.
 Proof. 
-  move => T tree.
-  elim: tree => //.
+  by move => T; case.
 Qed.
 
 Lemma height_subtrees : forall {T} (tree : BinaryTree T),
-  tree <> Nill T -> height tree = 1 + maxn (height (Lst tree)) (height (Rst tree)).
+  tree <> Nill T <-> height tree = 1 + maxn (height (Lst tree)) (height (Rst tree)).
 Proof.
-  move => T tree.
-  elim: tree => [| Ltree iHl value Rtree iHr HNill] // /=.
+  by move => T; case.
 Qed.
 
 (* Count of BinaryTree T *)
@@ -72,8 +84,17 @@ Fixpoint count {T} (tree : BinaryTree T) : nat :=
     | Node _ Left _ Right => 1 + (count Left) + (count Right)
     end.
 
-Eval compute in (count (Nill nat)).
-Eval compute in (count (Node (Nill nat) (Nill nat) 5 (Nill nat))).
+Eval compute in (height null).
+Eval compute in (count null).
+
+Eval compute in (height (@5)).
+Eval compute in (count (@5)).
+
+Eval compute in (height ((@3) -| 5 |- (@7))).
+Eval compute in (count ((@3) -| 5 |- (@7))).
+
+Eval compute in (height ((@3) -| 5 |- ((@6) -| 7 |- (@8)))).
+Eval compute in (count ((@3) -| 5 |- ((@6) -| 7 |- (@8)))).
 
 Lemma count_nill : forall {T}, count (Nill T) = 0.
 Proof.
@@ -83,15 +104,13 @@ Qed.
 Lemma count_empty_tree : forall {T} (tree : BinaryTree T),
   count tree = 0 <-> tree = Nill T.
 Proof.
-  move => T tree.
-  elim: tree => //.
+  by move => T; case.
 Qed.
 
 Lemma count_subtrees : forall {T} (tree : BinaryTree T),
-  tree <> Nill T -> count tree = 1 + count (Lst tree) + count (Rst tree).
+  tree <> Nill T <-> count tree = 1 + count (Lst tree) + count (Rst tree).
 Proof.
-  move => T tree.
-  elim: tree => //.
+  by move => T; case.
 Qed.
 
 (* =================================================== *)
@@ -101,8 +120,7 @@ Qed.
 Theorem leq_height_count : forall {T} (tree : BinaryTree T),
   height tree <= count tree.
 Proof.
-  move => T tree.
-  elim: tree => [| _ _ Ltree iHl value Rtree iHr] // /=.
+  move => T; elim => [| _ _ Ltree iHl value Rtree iHr] /= //.
 
     rewrite (leq_add2l 1 _ (_ + _)).
 
@@ -154,321 +172,9 @@ Proof.
     apply: leq_maxn_sum.
 Qed.
 
-(* ================== *)
-(* Binary search tree *)
-(* ================== *)
-
-Notation null := (Nill nat).
-Notation "l -| v |- r" := (Node (Nill nat) l v r) (at level 43, left associativity).
-Notation "@ v " := (null -| v |- null) (at level 43, left associativity).
-
-Check (@ 4).
-Check ((@3) -| 5 |- (@6)).
-
-Variable x : nat.
-
-Fixpoint Is_cond (s : seq nat) (P : nat -> bool) : bool :=
-  match s with 
-  | [::]    => true
-  | y :: ys => P y && Is_cond ys P
-  end.
-
-Fixpoint Left_cond (tree : BinaryTree nat) : bool := 
-  match tree with
-  | Nill => true
-  | Node _ Left value Right => (Is_cond (nodes (Lst tree)) (fun y => y < value))
-    && Left_cond Left && Left_cond Right
-  end.
-
-Fixpoint Right_cond (tree : BinaryTree nat) : bool := 
-  match tree with
-  | Nill => true
-  | Node _ Left value Right => Is_cond (nodes (Rst tree)) (fun y => value < y)
-    && Right_cond Left && Right_cond Right
-  end.
-
-Inductive BST : BinaryTree nat -> Prop :=
-  | bst_nill : BST null
-  | bst_node : forall tree, Left_cond tree -> Right_cond tree ->
-    BST (Lst tree) -> BST (Rst tree) -> BST tree.
-
-Eval compute in (Left_cond (((@1) -| 2 |- (@3)) -| 4 |- (@ 6))).
-Eval compute in (Left_cond (((@3) -| 2 |- (@1)) -| 4 |- (@ 6))).
-Eval compute in (Right_cond (((@1) -| 2 |- (@3)) -| 4 |- (@ 6))).
-Eval compute in (Right_cond (((@3) -| 2 |- (@1)) -| 4 |- (@ 6))).
-
 Ltac solve :=
   do ![try case: andP => //; case];
   try split => //; try done.
-
-Lemma BST_Nill : BST null.
-Proof.
-  apply: bst_nill.
-Qed.
-
-Lemma BST_Combine : forall tp tl v tr,
-  Left_cond (Node tp tl v tr) -> Right_cond (Node tp tl v tr) -> 
-  BST tl -> BST tr -> BST (Node tp tl v tr).
-Proof.
-  move => tp tl value tr Lc Rc lH rH.
-  by apply: bst_node.
-Qed.
-
-Lemma BST_One : forall y, BST (@ y).
-Proof.
-  move => y.
-  apply: bst_node => //.
-  - apply: BST_Nill.
-  - apply: BST_Nill.
-Qed.
-
-Lemma BST_Example_1 : BST ((@3) -| 5 |- (@ 7)).
-Proof.
-  apply: bst_node => // /=.
-  - apply: BST_One.
-  - apply: BST_One.
-Qed.
-
-Lemma BST_Two_l : forall a b, b < a -> 
-  BST ((@ b) -| a |- null).
-Proof.
-  move => a b cond.
-  apply: bst_node => // /=.
-  - solve.
-  - apply: BST_One.
-  - apply: BST_Nill.
-Qed.
-
-Lemma BST_Two_r : forall a b, a < b -> 
-  BST (null -| a |- (@ b)).
-Proof.
-  move => a b cond.
-  apply: bst_node => // /=.
-  - solve.
-  - apply: BST_Nill.
-  - apply: BST_One.
-Qed.
-
-Lemma BST_Tree : forall a b c, b < a < c -> 
-  BST ((@ b) -| a |- (@ c)).
-Proof.
-  move => a b c cond.
-  apply: bst_node => /=.
-  - solve.
-    by case: andP cond => //; case.
-  - solve.
-    by case: andP cond => //; case.
-  - apply: BST_One.
-  - apply: BST_One.
-Qed.
-
-Lemma BST_Example_2 : BST ((null -| 3 |- (@ 4)) -| 5 |- (@ 7)).
-Proof.
-  apply: bst_node => // /=.
-  - by apply: BST_Two_r.
-  - apply: BST_One.
-Qed.
-
-(* ============= *)
-(* Insert in BST *)
-(* ============= *)
-
-Fixpoint BST_insert (value : nat) (tree : BinaryTree nat) : BinaryTree nat :=
-    match tree with
-    | Nill                => null -| value |- null
-    | Node _ Left y Right =>
-        if value < y
-        then (BST_insert value Left) -| y |- Right
-        else if y < value 
-        then Left -| y |- (BST_insert value Right)
-        else tree
-    end.
-
-Notation "v >> t" := (BST_insert v t) (at level 43, left associativity).
-
-Eval compute in (2 >> null).
-Eval compute in (2 >> (@ 3)).
-Eval compute in (2 >> (@ 1)).
-Eval compute in (1 >> ((@ 2) -| 4 |- (@ 6))).
-Eval compute in (3 >> ((@ 2) -| 4 |- (@ 6))).
-Eval compute in (5 >> ((@ 2) -| 4 |- (@ 6))).
-Eval compute in (7 >> ((@ 2) -| 4 |- (@ 6))).
-
-Axiom Insert_cond : forall value tree, 
-  nodes (value >> tree) = value :: (nodes tree).
-
-Lemma Lst_elem : forall (tp tl tr : BinaryTree nat) v, Lst (Node tp tl v tr) = tl.
-Proof.
-  done.
-Qed.
-
-Lemma Rst_elem : forall (tp tl tr : BinaryTree nat) v, Rst (Node tp tl v tr) = tr.
-Proof.
-  done.
-Qed.
-
-Lemma Safety_Left_cond : forall tree y, Left_cond tree -> Left_cond (y >> tree).
-Proof.
-  elim => /= [y _ | tp _ tl iHtl z tr iHtr w H] //.
-  - case: andP H => //; case; solve => condL lH _ rH _.
-    case: (ltngtP w z) => cond /=; solve.
-    - rewrite Insert_cond => /=; solve.
-    - apply: iHtl lH.
-    - apply: iHtr rH.
-Qed.
-
-Lemma Safety_Right_cond : forall tree y, Right_cond tree -> Right_cond (y >> tree).
-Proof.
-  elim => /= [y _ | tp _ tl iHtl z tr iHtr w H] //.
-  - case: andP H => //; case; solve => condR lH _ rH _.
-    case: (ltngtP w z) => cond /=; solve.
-    - apply: iHtl lH.
-    - apply: iHtr rH.
-    - rewrite Insert_cond => /=.
-      by solve; apply: ltnW.
-Qed.
-
-Theorem Safety_BST_insert : forall tree y, BST tree -> BST (y >> tree).
-Proof.
-  elim => /= [y _ | tp _ tl iHtl z tr iHtr w H] //.
-  - apply: BST_One.
-    inversion H.
-    inversion H0; case: andP H6 => //; case.
-    case: andP => //; case => condL lH _ rH _;
-    inversion H1; case: andP H6 => //; case.
-    case: andP => //; case => condR lH' _ rH' _.
-    case: (ltngtP w z) => cond //.
-    - apply: BST_Combine => /= //.
-      - solve.
-        - rewrite Insert_cond => /=; solve.
-        - apply: Safety_Left_cond lH.
-      - solve.
-        apply: Safety_Right_cond lH'.
-      - apply: iHtl H2.
-    - apply: BST_Combine => /= //.
-      - solve; apply: Safety_Left_cond rH.
-      - solve.
-        - apply: Safety_Right_cond rH'.
-        - rewrite Insert_cond => /=.
-          by solve; apply: ltnW.
-      - apply: iHtr H3.
-Qed.
-
-(* ======================== *)
-(* BST with bool definition *)
-(* ======================== *)
-
-Fixpoint BST' (tree : BinaryTree nat) : bool := 
-  match tree with
-  | Nill => true
-  | Node _ Left value Right => 
-    Left_cond tree && Right_cond tree &&
-    BST' Left && BST' Right
-  end.
-
-Lemma BST'_Nill : BST' null.
-Proof.
-  done.
-Qed.
-
-Lemma BST'_Combine : forall tp tl v tr,
-  Left_cond (Node tp tl v tr) -> Right_cond (Node tp tl v tr) -> 
-  BST' tl -> BST' tr -> BST' (Node tp tl v tr).
-Proof.
-  move => /= tp tl value tr Lc Rc lH rH.
-  case: andP => //; case.
-  case: andP => //; case.
-  by case: andP => //; case.
-Qed.
-
-Lemma BST'_One : forall y, BST' (null -| y |- null).
-Proof.
-  done.
-Qed.
-
-Lemma BST'_Example_1 : BST' ((@ 3) -| 5 |- (@ 7)).
-Proof.
-  done.
-Qed.
-
-Lemma BST'_Two_l : forall a b, b < a -> 
-  BST' ((@ b) -| a |- null).
-Proof.
-  move => /= a b cond.
-  solve.
-Qed.
-
-Lemma BST'_Two_r : forall a b, a < b -> 
-  BST' (null -| a |- (@ b)).
-Proof.
-  move => /= a b cond; solve.
-Qed.
-
-Lemma BST'_Tree : forall a b c, b < a < c -> 
-  BST' ((@ b) -| a |- (@ c)).
-Proof.
-  move => /= a b c cond; solve.
-  - by case: andP cond => //; case.
-  - by case: andP cond => //; case.
-Qed.
-
-Lemma BST'_Example_2 : BST' ((null -| 3 |- (@ 4)) -| 5 |- (@ 7)).
-Proof.
-  done.
-Qed.
-
-Theorem Safety_BST'_insert : forall tree y, BST' tree -> BST' (y >> tree).
-Proof.
-  elim => /= [y _ | tp _ tl iHtl z tr iHtr w] //.
-  case: andP => //; case.
-  case: andP => //; case.
-  case: andP => //; case => condL condR _ lH _ rH _.
-  case: andP condR => //; case.
-  case: andP => //; case => condtR LH _ RH _.
-  case: andP condL => //; case.
-  case: andP => //; case => condtL LH' _ RH' _.
-  case: (ltngtP w z) => cond /= //. 
-  - rewrite Insert_cond /=; solve.
-    - apply: iHtl lH.
-    - apply: Safety_Right_cond LH.
-    - apply: Safety_Left_cond LH'.
-  - rewrite Insert_cond /=; solve.
-    - apply: iHtr rH.
-    - apply: Safety_Right_cond RH.
-    - apply: Safety_Left_cond RH'.
-  solve.
-Qed.
-
-(* =========================== *)
-(* Reflect betwen BST and BST' *)
-(* =========================== *)
-
-Lemma bstP (tree : BinaryTree nat) : reflect (BST tree) (BST' tree).
-Proof.
-  elim: tree => [| tp _ tl iHtl z tr iHtr] /=.
-  - constructor; apply: BST_Nill.
-  - case: andP.
-    - case; case: andP => //; case.
-      case; case: andP => //. case => condL condR _ lH _ rH;
-      constructor.
-      apply: BST_Combine => //.
-      - by case: iHtl lH.
-      - by case: iHtr rH.
-    - move => H1. constructor. move => H2.
-      apply: H1. inversion H2.
-      case: andP => //; case.
-      - solve. move: H3.
-        rewrite Rst_elem. case: iHtr => //.
-      - case: andP => //; case.
-        - split => //. move: H1.
-          rewrite Lst_elem; case: iHtl => //.
-        - split => //.
-Qed.
-
-Lemma BST_Example_3 : BST (((@2) -| 3 |- (@ 4)) -| 5 |- ((@6) -| 7 |- (@ 9))).
-Proof.
-  by apply: bstP.
-Qed.
 
 (* ============================================================ *)
 (* ### ----- Canonical comparison and eqType for BynaryTree T.  *)
@@ -525,6 +231,296 @@ Eval compute in (null == (@4) -| 5 |- (@6)).
 Eval compute in ((@4) -| 5 |- (@6) == (@4) -| 5 |- (@6)).
 Eval compute in ((@3) -| 5 |- (@6) == (@4) -| 5 |- (@6)).
 
+(* ================== *)
+(* Binary search tree *)
+(* ================== *)
+
+Fixpoint Is_cond (s : seq nat) (P : nat -> bool) : bool :=
+  match s with 
+  | [::]    => true
+  | y :: ys => P y && Is_cond ys P 
+  end.
+
+Fixpoint Left_cond (tree : BinaryTree nat) : bool := 
+  match tree with
+  | Nill => true
+  | Node _ Left value Right => Is_cond (nodes (Lst tree)) (fun y => y < value)
+    && Left_cond Left && Left_cond Right
+  end.
+
+Fixpoint Right_cond (tree : BinaryTree nat) : bool := 
+  match tree with
+  | Nill => true
+  | Node _ Left value Right => Is_cond (nodes (Rst tree)) (fun y => value < y)
+    && Right_cond Left && Right_cond Right
+  end.
+
+Eval compute in (Left_cond (((@1) -| 2 |- (@3)) -| 4 |- (@ 6))).
+Eval compute in (Left_cond (((@3) -| 2 |- (@1)) -| 4 |- (@ 6))).
+Eval compute in (Right_cond (((@1) -| 2 |- (@3)) -| 4 |- (@ 6))).
+Eval compute in (Right_cond (((@3) -| 2 |- (@1)) -| 4 |- (@ 6))).
+
+Inductive BST : BinaryTree nat -> Prop :=
+  | bst_nill : BST null
+  | bst_node : forall tree, Left_cond tree -> Right_cond tree ->
+    BST (Lst tree) -> BST (Rst tree) -> BST tree.
+
+Lemma BST_Nill : BST null.
+Proof.
+  apply: bst_nill.
+Qed.
+
+Lemma BST_Combine : forall tp tl v tr,
+  Left_cond (Node tp tl v tr) -> Right_cond (Node tp tl v tr) -> 
+  BST tl -> BST tr -> BST (Node tp tl v tr).
+Proof.
+  move => tp tl value tr Lc Rc lH rH.
+  by apply: bst_node.
+Qed.
+
+Lemma BST_One : forall y, BST (@ y).
+Proof.
+  move => y;
+  apply: bst_node => //;
+  do [apply: BST_Nill]. 
+Qed.
+
+Lemma BST_Example_1 : BST ((@3) -| 5 |- (@ 7)).
+Proof.
+  apply: bst_node => //;
+  do [apply: BST_One].
+Qed.
+
+Lemma BST_Two_l : forall a b, b < a -> 
+  BST ((@ b) -| a |- null).
+Proof.
+  move => a b cond.
+  apply: bst_node => // /=.
+  - solve.
+  - apply: BST_One.
+  - apply: BST_Nill.
+Qed.
+
+Lemma BST_Two_r : forall a b, a < b -> 
+  BST (null -| a |- (@ b)).
+Proof.
+  move => a b cond.
+  apply: bst_node => // /=.
+  - solve.
+  - apply: BST_Nill.
+  - apply: BST_One.
+Qed.
+
+Lemma BST_Tree : forall a b c, b < a < c -> 
+  BST ((@ b) -| a |- (@ c)).
+Proof.
+  move => a b c cond.
+  apply: bst_node => /=.
+  - solve.
+    by case: andP cond => //; case.
+  - solve.
+    by case: andP cond => //; case.
+  - apply: BST_One.
+  - apply: BST_One.
+Qed.
+
+Lemma BST_Example_2 : BST ((null -| 3 |- (@ 4)) -| 5 |- (@ 7)).
+Proof.
+  by apply: bst_node => //;
+  do [apply: BST_Two_r| apply: BST_One].
+Qed.
+
+(* ============= *)
+(* Insert in BST *)
+(* ============= *) 
+
+Fixpoint BST_insert (value : nat) (tree : BinaryTree nat) : BinaryTree nat :=
+    match tree with
+    | Nill                => null -| value |- null
+    | Node _ Left y Right =>
+        if value < y
+        then (BST_insert value Left) -| y |- Right
+        else if y < value 
+        then Left -| y |- (BST_insert value Right)
+        else tree
+    end. 
+
+Notation "v >> t" := (BST_insert v t) (at level 43, left associativity).
+
+Eval compute in (2 >> null).
+Eval compute in (2 >> (@ 3)).
+Eval compute in (2 >> (@ 1)).
+Eval compute in (1 >> ((@ 2) -| 4 |- (@ 6))).
+Eval compute in (3 >> ((@ 2) -| 4 |- (@ 6))).
+Eval compute in (5 >> ((@ 2) -| 4 |- (@ 6))).
+Eval compute in (7 >> ((@ 2) -| 4 |- (@ 6))).
+
+Axiom Insert_cond : forall value tree, 
+  nodes (value >> tree) = value :: (nodes tree).
+
+Lemma Safety_Left_cond : forall tree y, Left_cond tree -> Left_cond (y >> tree).
+Proof.
+  elim => /= [y _ | tp _ tl iHtl z tr iHtr w H] //.
+  - case: andP H => //; case; solve => condL lH _ rH _.
+    case: (ltngtP w z) => cond /=; solve.
+    - rewrite Insert_cond => /=; solve.
+    - apply: iHtl lH.
+    - apply: iHtr rH.
+Qed.
+
+Lemma Safety_Right_cond : forall tree y, Right_cond tree -> Right_cond (y >> tree).
+Proof.
+  elim => /= [y _ | tp _ tl iHtl z tr iHtr w H] //.
+  - case: andP H => //; case; solve => condR lH _ rH _.
+    case: (ltngtP w z) => cond /=; solve.
+    - apply: iHtl lH.
+    - apply: iHtr rH.
+    - rewrite Insert_cond => /=.
+      by solve; apply: ltnW.
+Qed.
+
+Theorem Safety_BST_insert : forall tree y, BST tree -> BST (y >> tree).
+Proof.
+  elim => /= [y _ | tp _ tl iHtl z tr iHtr w H] //.
+  - apply: BST_One.
+    inversion H.
+    inversion H0; case: andP H6 => //; case.
+    case: andP => //; case => condL lH _ rH _;
+    inversion H1; case: andP H6 => //; case.
+    case: andP => //; case => condR lH' _ rH' _.
+    case: (ltngtP w z) => cond //.
+    - apply: BST_Combine => /= //.
+      - solve.
+        - rewrite Insert_cond => /=; solve.
+        - apply: Safety_Left_cond lH.
+      - solve.
+        apply: Safety_Right_cond lH'.
+      - apply: iHtl H2.
+    - apply: BST_Combine => /= //.
+      - solve; apply: Safety_Left_cond rH.
+      - solve.
+        - apply: Safety_Right_cond rH'.
+        - rewrite Insert_cond => /=.
+          by solve; apply: ltnW.
+      - apply: iHtr H3.
+Qed.
+
+(* ======================== *)
+(* BST with bool definition *)
+(* ======================== *)
+
+Fixpoint BSTeq (tree : BinaryTree nat) : bool := 
+  match tree with
+  | Nill => true
+  | Node _ Left value Right => 
+    Left_cond tree && Right_cond tree &&
+    BSTeq Left && BSTeq Right
+  end.
+
+Lemma BSTeq_Nill : BSTeq null.
+Proof.
+  done.
+Qed.
+
+Lemma BSTeq_Combine : forall tp tl v tr,
+  Left_cond (Node tp tl v tr) -> Right_cond (Node tp tl v tr) -> 
+  BSTeq tl -> BSTeq tr -> BSTeq (Node tp tl v tr).
+Proof.
+  move => /= tp tl value tr Lc Rc lH rH.
+  case: andP => //; case.
+  case: andP => //; case.
+  by case: andP => //; case.
+Qed.
+
+Lemma BSTeq_One : forall y, BSTeq (null -| y |- null).
+Proof.
+  done.
+Qed.
+
+Lemma BSTeq_Example_1 : BSTeq ((@ 3) -| 5 |- (@ 7)).
+Proof.
+  done.
+Qed.
+
+Lemma BSTeq_Two_l : forall a b, b < a -> 
+  BSTeq ((@ b) -| a |- null).
+Proof.
+  move => /= a b cond.
+  solve.
+Qed.
+
+Lemma BSTeq_Two_r : forall a b, a < b -> 
+  BSTeq (null -| a |- (@ b)).
+Proof.
+  move => /= a b cond; solve.
+Qed.
+
+Lemma BSTeq_Tree : forall a b c, b < a < c -> 
+  BSTeq ((@ b) -| a |- (@ c)).
+Proof.
+  move => /= a b c cond; solve.
+  - by case: andP cond => //; case.
+  - by case: andP cond => //; case.
+Qed.
+
+Lemma BSTeq_Example_2 : BSTeq ((null -| 3 |- (@ 4)) -| 5 |- (@ 7)).
+Proof.
+  done.
+Qed.
+
+Theorem Safety_BSTeq_insert : forall tree y, BSTeq tree -> BSTeq (y >> tree).
+Proof.
+  elim => /= [y _ | tp _ tl iHtl z tr iHtr w] //.
+  case: andP => //; case.
+  case: andP => //; case.
+  case: andP => //; case => condL condR _ lH _ rH _.
+  case: andP condR => //; case.
+  case: andP => //; case => condtR LH _ RH _.
+  case: andP condL => //; case.
+  case: andP => //; case => condtL LH' _ RH' _.
+  case: (ltngtP w z) => cond /= //. 
+  - rewrite Insert_cond /=; solve.
+    - apply: iHtl lH.
+    - apply: Safety_Right_cond LH.
+    - apply: Safety_Left_cond LH'.
+  - rewrite Insert_cond /=; solve.
+    - apply: iHtr rH.
+    - apply: Safety_Right_cond RH.
+    - apply: Safety_Left_cond RH'.
+  solve.
+Qed.
+
+(* =========================== *)
+(* Reflect betwen BST and BST' *)
+(* =========================== *)
+
+Theorem bstP (tree : BinaryTree nat) : reflect (BST tree) (BSTeq tree).
+Proof.
+  elim: tree => [| tp _ tl iHtl z tr iHtr] /=.
+  - constructor; apply: BST_Nill.
+  - case: andP.
+    - case; case: andP => //; case.
+      case; case: andP => //. case => condL condR _ lH _ rH.
+      constructor.
+      apply: BST_Combine => //.
+      - by case: iHtl lH.
+      - by case: iHtr rH.
+    - move => H1. constructor. move => H2.
+      apply: H1. inversion H2.
+      case: andP => //; case.
+      - solve. move: H3.
+        rewrite Rst_elem. case: iHtr => //.
+      - case: andP => //; case.
+        - split => //. move: H1.
+          rewrite Lst_elem; case: iHtl => //.
+        - split => //.
+Qed.
+
+Lemma BST_Example_3 : BST (((@2) -| 3 |- (@ 4)) -| 5 |- ((@6) -| 7 |- (@ 9))).
+Proof.
+  by apply: bstP.
+Qed.
+
 (* =========================== *)
 (* ### ----- Tree with parents *)
 (* =========================== *)
@@ -555,12 +551,12 @@ Fixpoint Parent_cond {T: eqType} (tree : BinaryTree T) : bool :=
 Inductive BSTwP : BinaryTree nat -> Prop :=
   | wP_constr : forall tree, BST tree -> Parent_cond tree -> BSTwP tree.
 
-Definition BSTwP' (tree : BinaryTree nat) : bool :=
-  BST' tree && Parent_cond tree.
+Definition BSTwPeq (tree : BinaryTree nat) : bool :=
+  BSTeq tree && Parent_cond tree.
 
-Lemma bstwpP (tree : BinaryTree nat) : reflect (BSTwP tree) (BSTwP' tree).
+Lemma bstwpP (tree : BinaryTree nat) : reflect (BSTwP tree) (BSTwPeq tree).
 Proof.
-  unfold BSTwP'.
+  unfold BSTwPeq.
   case: andP => cond; constructor.
   - constructor; case: cond => //;
     case: bstP => //.
@@ -594,7 +590,7 @@ Axiom Insert_cond_wP : forall value tree,
   nodes (value >>wP tree) = value :: (nodes tree).
 
 Lemma bst_insertP (tree : BinaryTree nat) (y : nat) : 
-  reflect (BST' (y >> tree)) (BST' (y >>wP tree)).
+  reflect (BSTeq (y >> tree)) (BSTeq (y >>wP tree)).
 Proof.
   elim: tree y => [| tp iHtp tl iHtl v tr iHtr y] /=; 
         do [by constructor|].
